\documentclass[twocolumn,8pt]{extarticle}
\usepackage[english]{babel} 
\usepackage[latin1]{inputenc} 
\usepackage{times}			% Default times font style
\usepackage[T1]{fontenc} 	% Font encoding
\usepackage{amsmath} 		% Math package
\usepackage{mathtools} 		% Adds the declare paired 
							% delimeter command to make costom \abs and \norm
\usepackage{breqn}		 	% Adds dmath environment for automated brakeline
\usepackage{xfrac}			% Adds slanted fractions (sfrac)
\usepackage{cancel}			% Adds the cancel command, a slash through the symbol(s)
\usepackage{tabularx}		% Adds adjustable width on tabulars
\usepackage{cuted}			% Adds the strip command, pagewidth text in a twocolumn
							% environment. 
\usepackage{hyperref}

% Start custom \abs \norm 
\DeclarePairedDelimiter\abs{\lvert}{\rvert}%
\DeclarePairedDelimiter\norm{\lVert}{\rVert}%
% Swap the definition of \abs* and \norm*, so that \abs
% and \norm resizes the size of the brackets, and the 
% starred version does not.
\makeatletter
\let\oldabs\abs
\def\abs{\@ifstar{\oldabs}{\oldabs*}}
%
\let\oldnorm\norm
\def\norm{\@ifstar{\oldnorm}{\oldnorm*}}
\makeatother
% End costum \abs \norm 

% TODO: Put comments on this section.
\newcommand{\eq}[1]{{\small\begin{align*}#1\end{align*}}}
\newcommand{\equ}[1]{{\small\begin{align}#1\end{align}}}
\newcommand{\mat}[1]{\begin{matrix}#1\end{matrix}}
\renewcommand\vec[1]{\mathbf{#1}}
\newcommand{\OP}[1]{\mathbf{\widehat{#1}}}
\newcommand{\op}[1]{\hat{#1}}
\newcommand{\unit}[1]{\mathbf{\hat{#1}}}

\title{}

\begin{document}

\begin{titlepage}
\begin{center}

\textsc{\Large Variational Monte Carlo Simulations of
Atomic Systems}\\[0.5cm]
\rule{\linewidth}{0.5mm} \\[0.4cm]
{ \huge \bfseries  Part I}\\[0.10cm]
\rule{\linewidth}{0.5mm} \\[1.5cm]
\textsc{\Large FYS4411}\\
\textsc{\Large Computational Physics II}\\[1.5cm]
\textsc{}\\[1.5cm]

% Av hvem?
\begin{minipage}{0.49\textwidth}
    \begin{center} \large
		Daniel Marelius Bj\o rnstad
    \end{center}
\end{minipage}
\begin{minipage}{0.49\textwidth}
    \begin{center} \large
        Alexander Fleischer
    \end{center}
\end{minipage}

\vfill

% Dato nederst
\large{Dato: \today}

\end{center}
\end{titlepage}

\maketitle
%\newpage

\section{Introduction}
Github: \\ \url{https://github.com/lastis/FYS4411}

\section{Methods}
\subsection{Trial Wavefunction of Beryllium}

The trial wavefunction of Beryllium ca be written on the form
\equ{
  \psi_{T}(\vec r_1, \vec r_2, \vec r_3, \vec r_4) = \psi_{D}\psi_{C} \label{psiT}
}
where the Slater determinant is
\equ{
  \psi_D &= Det\left(\phi_{1}(\vec r_1),\phi_{2}(\vec r_2),
    \phi_{3}(\vec r_3),\phi_{4}(\vec r_4)\right) \label{psiD}\\
  &= \left(\phi_{1s}^1\phi_{2s}^2
    -\phi_{1s}^2\phi_{2s}^1\right)
    \left(\phi_{1s}^3\phi_{2s}^4
    -\phi_{1s}^4\phi_{2s}^3\right)\nonumber
}
and the correlations part is
\equ{
  \psi_C = \prod_{i<j}^{4}\exp{\left(\frac{ar_{ij}}{2(1+\beta r_{ij})}\right)} \label{psiC}
}
Here $\phi_i(\vec r_i)$ are the hydrogen-like wavefunctions. They are given by
the $1s$ and $2s$ orbital parts
\eq{                                                               
\phi_{1s}^i &= e^{-\alpha r_i}                                   
}
and
\eq{
  \phi_{2s}^i &= \left(1-\alpha r_i/2\right)e^{-\alpha r_i/2}
}
which are dependent on the vectors $\vec r_i$.

We want to determine the local energy $E_L$ to approximate
the ground state energy of the atom.
The general expression for the local energy is
\eq{
  E_L = \frac{1}{\psi_T (\vec R)}\OP H \psi_T (\vec R) 
}
and the Hamiltonian can generally be described as a sum of the contributions
to the potential energy by the electron-electron repulsion and the nucleus-electron interaction, aswell as the kinetic energy. This gives us a Hamiltonian on the form
\eq{
  \OP H &= \OP K + \OP V \\
  &=\sum_i (\op k_i + \op v_i)  + \sum_{i<j} \op v_{ij}\\
  &= -\sum_{i=1}^N\bigg[
    \frac{\op\nabla_i^2}{2} + \frac{2}{r_i}\bigg] 
  + \sum_{i=1}^{N-1}\sum_{j=i+1}^N\frac{1}{r_{ij}}
}
From this expression, it's clear that $\OP K$ is the only operator that changes the
trial wavefunction when we calculate the local energy. Therefore, we must calculate the
following quantities
\eq{
  \frac{1}{\psi_T}\op k_i \psi_T = -\frac{1}{2}\frac{\op\nabla_i^2 \psi_T}{\psi_T}
}
For Beryllium, the trial wavefunction is a product of the Slater determinant part 
and the correlations part, namely $\psi_T = \psi_D\psi_C$.

The product rule of differentiation gives us
\eq{
  \frac{\op\nabla^2 \psi_T}{\psi_T} = 
  \frac{\op\nabla^2 \psi_D}{\psi_D}
    +2 \frac{\op\nabla \psi_D}{\psi_D}\cdot\frac{\op\nabla \psi_C}{\psi_C}
    +\frac{\op\nabla^2 \psi_C}{\psi_C}
}

We start by finding the first and second derivative of the determinant part,
which are only dependent on the radii of the particles. This means that the gradient can be written 
\eq{
  \nabla f = \unit r \frac{\partial f}{\partial r}
  \;\text{ and }\;
  \nabla^2 f = \frac{\partial^2 f}{\partial r^2} 
    + \frac{2}{r}\frac{\partial f}{\partial r}
}
where $\vec r = r\unit r$.
  
First we define
the following
\eq{
  f_i &\equiv -\frac{\alpha \vec r_i}{2}\\
  g_i &\equiv \exp(f_i)\\
  F_{ij} &\equiv \phi_{1s}(\vec r_i)\phi_{2s}(\vec r_j)
  -\phi_{1s}(\vec r_j)\phi_{2s}(\vec r_i)
}
We then have
\eq{
  \phi_{1s}^i &= g_i^2\\
  \frac{\partial \phi_{1s}^i}{\partial r_i} &= -\alpha g_i^2\\
  \frac{\partial^2 \phi_{1s}^i}{\partial r_i^2} &= \alpha^2 g_i^2\\
  \phi_{2s}^i &= g_i(1+f_i)\\
  \frac{\partial \phi_{2s}^i}{\partial r_i} &= -\alpha g_i(1+f_i/2)\\
  \frac{\partial^2 \phi_{2s}^i}{\partial r_i^2} &= \frac{3\alpha^2}{4} g_i(1+f_i/3)
}
so we get
\eq{
  F_{ij} &= g_i^2 (1+f_j)g_j - g_j^2 (1+f_i)g_i\\
  \frac{\partial F_{ij}}{\partial r_i} 
    &= -\alpha g_i g_j (g_i(1+f_j) - g_j (1+f_i/2))\\
  \frac{\partial^2 F_{ij}}{\partial r_i^2} 
    &= \alpha^2 g_i g_j (g_i(1+f_j) - \frac{3}{4} g_j (1+f_i/3))\\
  \frac{\partial F_{ij}}{\partial r_j} 
    &= \alpha g_i g_j (g_j(1+f_i) - g_i (1+f_j/2))\\
  \frac{\partial^2 F_{ij}}{\partial r_j^2} 
    &= -\alpha^2 g_i g_j (g_j(1+f_i) - \frac{3}{4} g_i (1+f_j/3))\\
}
The determinant part is
\eq{
  \psi_D = F_{12}F_{34}
}
where the first is only affected by differentiation with respect to particle 1 or 2,
and opposite for the second part
\eq{
  \mat{
    \frac{\op\nabla_1 \psi_D}{\psi_D} = \frac{\op\nabla_1 F_{12}}{F_{12}} &
    \frac{\op\nabla_2 \psi_D}{\psi_D} = \frac{\op\nabla_2 F_{12}}{F_{12}} \\\\
    \frac{\op\nabla_3 \psi_D}{\psi_D} = \frac{\op\nabla_3 F_{34}}{F_{34}} &
    \frac{\op\nabla_4 \psi_D}{\psi_D} = \frac{\op\nabla_4 F_{34}}{F_{34}}
  }
}
The result is two different quantities
\eq{
  \frac{\op\nabla_k \psi_D}{\psi_D} =
  \begin{cases}
    \frac{\op\nabla_i F_{ij}}{F_{ij}}
    &= -\alpha \frac{\vec r_i}{r_i} \frac{(g_i(1+f_j) 
      - g_j (1+f_i/2))}{g_i (1+f_j) - g_j (1+f_i)}
    ,\text{ if } k=i=j-1 \\\\
    \frac{\op\nabla_j F_{ij}}{F_{ij}}
    &= -\alpha \frac{\vec r_j}{r_j}\frac{(g_i (1+f_j/2) 
      - g_j(1+f_i))}{g_i (1+f_j) - g_j (1+f_i)}
    ,\text{ if } k=j=i+1
  \end{cases}
}
one for particles 1 and 3, and one for 2 and 4, where $i\in {1,3}$ and $j\in {2,4}$.

For the second derivative part, we have 
\eq{
  \frac{\op\nabla_k^2 \psi_D}{\psi_D} =
  \begin{cases}
    \frac{\op\nabla_i^2 F_{ij}}{F_{ij}}
    &= \frac{\alpha^2 (g_i(1+f_j) 
      - \frac{3}{4} g_j (1+f_i/3)) - \frac{2\alpha}{r}(g_i(1+f_j) - g_j (1+f_i/2))}
      {g_i (1+f_j) - g_j (1+f_i)}\\\\
    \frac{\op\nabla_j^2 F_{ij}}{F_{ij}}
    &= \frac{\alpha^2 (\frac{3}{4}g_i(1+f_j/3) 
      - g_j (1+f_i)) - \frac{2\alpha}{r}(g_i (1+f_j/2) 
      - g_j(1+f_i))}
      {g_i (1+f_j) - g_j (1+f_i)}
  \end{cases}
}
with the same conditions as above.

Now we move on to the calculation of the correlation parts (\ref{psiC}). First off, we define
\eq{
  f_{ij} \equiv \frac{ar_{ij}}{2(1+\beta r_{ij})}
}
The gradient of the wavefunction, 
divided by the wavefunction for particle, $k$ in the $x$-direction is then
\eq{
  \left[\frac{\nabla_k\psi_C}{\psi_C}\right]_x 
  =\frac{1}{\psi_C}\frac{\partial\psi_C}{\partial x_k}
}
If we look at the gradient, 
we see that the parts of the wavefunction that is not dependent on $k$, 
will not be affected by the differentiation, so
\equ{
  \frac{\partial\psi_C}{\partial x_k}=\prod_{i,j\neq k} g_{ij}
    \frac{\partial}{\partial x_k}
    \left[ \prod_{i<k} g_{ik} + \prod_{i>k} g_{ki} \right]\label{DpsiC}
}
Here we have split the espression for $i<k$ and $k>i$.

When we do the differentiation and divide by the wavefunction, we see that
\eq{
  \left[\frac{\nabla_k\psi_C}{\psi_C}\right]_x
  &=\sum_{i=1}^{k-1}\frac{1}{g_{ik}}\frac{\partial g_{ik}}{\partial x_k}  
  + \sum_{i=k+1}^{N}\frac{1}{g_{ki}}\frac{\partial g_{ki}}{\partial x_k} \\
  &=\sum_{i=1}^{k-1}\frac{\partial f_{ik}}{\partial x_k}  
  - \sum_{i=k+1}^{N}\frac{\partial f_{ki}}{\partial x_i}\\
  &=\sum_{i=1}^{k-1}\frac{x_k-x_i}{r_{ik}}\frac{\partial f_{ik}}{\partial r_{ik}}  
  - \sum_{i=k+1}^{N}\frac{x_i-x_k}{r_{ki}}\frac{\partial f_{ki}}{\partial r_{ki}}
}
since $g_{ij}$ is an exponential function, 
and $\frac{\partial}{\partial x_i}g_{ij} = -\frac{\partial}{\partial x_j}g_{ij}$.

Finally, we have used the chain rule to attain an expression that is dependent
on the distance between the two particles
\eq{
  \frac{\partial f_{ij}}{\partial x_j} 
  = \frac{\partial f_{ij}}{\partial r_{ij}} \frac{\partial r_{ij}}{\partial x_j} 
  = \frac{x_j - x_i}{r_{ij}} \frac{\partial f_{ij}}{\partial r_{ij}}
}
Thus
\eq{
  \frac{\nabla_k\psi_C}{\psi_C} &=
    \sum_{i=1}^{k-1}\frac{\vec r_{ik}}{r_{ik}}\frac{\partial f_{ik}}{\partial r_{ik}}  
    - \sum_{i=k+1}^{N}\frac{\vec r_{ki}}{r_{ki}}\frac{\partial f_{ki}}{\partial r_{ki}}\\
    &=\sum_{i=1}^{k-1}\frac{\vec r_{ik}}{r_{ik}}\frac{a}{2(1+\beta r_{ik})^2}  
    - \sum_{i=k+1}^{N}\frac{\vec r_{ki}}{r_{ki}}\frac{a}{2(1+\beta r_{ki})^2}\\
    &=\sum_{i\neq k}\frac{\vec r_{ki}}{r_{ki}}\frac{a}{2(1+\beta r_{ki})^2} 
}

From (\ref{DpsiC}), we can gather that the double derivative part is described by
\eq{
  \left[\frac{\mathbf{\nabla}^2 \Psi_C}{\Psi_C}\right]_x &=
  2\sum_{k=1}^{N}
    \sum_{i=1}^{k-1}\frac{\partial^2 f_{ik}}{\partial x_k^2}\ +\ 
    \sum_{k=1}^N
    \left(\sum_{i=1}^{k-1}\frac{\partial f_{ik}}{\partial x_k} -
    \sum_{i=k+1}^{N}\frac{\partial f_{ki}}{\partial x_i}
    \right)^2\\
  &=2
    \sum_{k=1}^{N}
    \sum_{i=1}^{k-1}\frac{\partial^2 g_{ik}}{\partial x_k^2}\ +\ 
    \sum_{k=1}^N
    \left(\sum_{i\neq k}\frac{\vec r_{ki}}{r_{ki}}\frac{a}{2(1+\beta r_{ki})^2} 
    \right)^2
}
\section{Results}

\end{document}